src/ListUtil.v
@@ -1,0 +1,29 @@
+Require Import Coq.Lists.List.
+
+Module FromNil.
+  Section WithElementType.
+    Context {A : Type}.
+    Definition nth_error_count l n : nat + A :=
+      fold_right (fun a s => match s with
+                             | inl n =>
+                               match n with
+                               | O => inr a
+                               | S n => inl n
+                               end
+                             | inr a => inr a
+                             end)
+                 (inl n) l.
+    Definition nth_error (l : list A) (n : nat) : option A :=
+      match nth_error_count l n with
+      | inl _ => None
+      | inr a => Some a
+      end.
+  End WithElementType.
+
+  Module _test.
+    Local Definition t0 : nth_error (2::1::0::nil) 0 = Some 0 := eq_refl.
+    Local Definition t1 : nth_error (2::1::0::nil) 1 = Some 1 := eq_refl.
+    Local Definition t2 : nth_error (2::1::0::nil) 2 = Some 2 := eq_refl.
+    Local Definition tx : nth_error (2::1::0::nil) 3 = None := eq_refl.
+  End _test.
+End FromNil.
